ported the invariants of outer loop. Stuck on the inability to talk about the contents of an entire array in the middle of an SST program. Of course, one can read the array in a loop, but it is senseless to do computation to enable reasoning about correctness.
While storing bitvectors
directly as functions, this was being done in "just one" wasted operation.

This problem needs serious thought. For now, added a crazy memreadAll function
that returns a hidden version of the whole memory.

Because its result is in SST, it might not get automatically erased

examples/low-level/sieve.fst
@@ -8,6 +8,7 @@ module Sieve
 open SSTCombinators
 open StackAndHeap
 open SST
+
 open Heap
 open Stack
 open Set
@@ -52,7 +53,7 @@ type markedIffMultipleOrInit (n:nat) (lo:nat) (upto:nat)
   /\ (forall (m:nat{m < n}). (marked n neww m ==> (marked n init m \/
       SieveFun.nonTrivialDivides lo m) ))
 
-type  innerLoopInv (n:nat) (lo: ref nat)  (li : ref nat) (res: (sstarray bool))
+type  innerLoopInv (n:nat) (lo: ref nat)  (li : ref nat) (res: bitarray)
     (initres: bitv n) (m:smem) =
  SieveFun.distinctRefsExists3 m lo (reveal (asRef res)) li
   /\ 1 < (loopkupRef li m) /\  haslength m res n
@@ -133,31 +134,54 @@ let innerLoop n lo li res initres =
     (*the part below has no computaional content; why does SMTPatT not work?*)
       //let newv = memread res in
       //let lov = memread lo in
-    (*  (multiplesMarkedAsDividesIff n initres newv lo) // how to invoke this lemma now? unlike previously, we cannot read a full Seq from an array
+    (*      (multiplesMarkedAsDividesIff n initres newv lo) // how to invoke this lemma now? unlike previously, we cannot read a full Seq from an array
     *)
 
-type  outerLoopInv (n:nat) (lo: ref nat) (res:ref ((k:nat{k<n}) -> Tot bool)) (m:smem) =
- distinctRefsExists2 m lo res
+type markedIffHasDivisorSmallerThan (n:nat) (lo:nat)
+    (neww: bitv n) =
+    (forall (k:nat{k < n}). (marked n neww k <==> (exists (d:nat{1<d}). d<lo /\ SieveFun.nonTrivialDivides d k)))
+
+
+val markedIffHasDivisorSmallerThanInc :
+  n:nat -> lo:nat{1<lo} -> old:(bitv n) -> neww:(erased (bitv n))
+  -> Lemma
+      (requires (markedIffHasDivisorSmallerThan n lo old)
+              /\ markedIffDividesOrInit2 n lo old (reveal neww))
+      (ensures (markedIffHasDivisorSmallerThan n (lo+1) (reveal neww)))
+      (*[SMTPatT (markedIffHasDivisorSmallerThan n (lo+1) neww)]*)
+let markedIffHasDivisorSmallerThanInc n lo old neww  = ((multiplesMarkedAsDividesIff n old neww lo))
+
+type allUnmarked
+   (n:nat) (neww: bitv n) =
+   forall (m:nat{m<n}). not (marked n neww m)
+
+type  outerLoopInv (n:nat) (lo: ref nat) (res: bitarray) (m:smem) =
+ SieveFun.distinctRefsExists2 m lo (reveal (asRef res))
   /\ (((loopkupRef lo m) - 1) < n)
-  /\ (1<(loopkupRef lo m))
-  /\ (markedIffHasDivisorSmallerThan n (loopkupRef lo m) (loopkupRef res m))
+  /\ (1<(loopkupRef lo m)) /\  haslength m res n
+  /\ (markedIffHasDivisorSmallerThan n (loopkupRef lo m) (reveal (esel m res)))
 
 
 (*#set-options "--initial_fuel 100 --max_fuel 10000 --initial_ifuel 100 --max_ifuel 10000"*)
 
+(*Danger!! this function is highly experimental*)
+assume val memreadAll : unit -> PureMem (erased smem)
+      (requires (fun m -> true))
+      (ensures (fun _ v m -> reveal v = m))
+
+
 val outerLoopBody :
   n:nat{n>1}
   -> lo:(ref nat)
-  -> res : ref ((k:nat{k<n}) -> Tot bool)
+  -> res : bitarray
   -> unit ->
   whileBody
     (outerLoopInv n lo res)
-    (outerGuardLC n lo)
-    (hide (union (singleton (Ref lo)) (singleton (Ref res))))
+    (SieveFun.outerGuardLC n lo)
+    ((elift2 union) (gonly lo)  (ArrayAlgos.eonly res))
 
 
 let outerLoopBody n lo res u =
-  (*pushStackFrame ();*)
   let initres = memread res in
   let lov = memread lo in
   let li = salloc 2 in
